Trace Equiv

theories/MP/GLTraceEquiv.v
@@ -16,10 +16,10 @@ Require Import MPST.MP.Projection.
 Section TraceEquiv.
 
   Definition step_equiv G P :=
-    forall a, exists G' P', step a G G' <-> lstep a P P'.
+    forall a, (exists G', step a G G') <-> (exists P', lstep a P P').
 
   Definition trace_equiv G P :=
-    forall a, exists G' P', g_lts a G G' <-> l_lts a P P'.
+    forall a, (exists G', g_lts a G G') <-> (exists P', l_lts a P P').
 
   Fixpoint add_head p (Q : MsgQ) :=
     match Q with
@@ -31,9 +31,31 @@ Section TraceEquiv.
   Notation msg m := (m.1, inr m.2).
   Notation lab m l := (m.1, inl l).
 
+  Fixpoint merge_mq (Q : MsgQ) (Qs : seq MsgQ) :=
+    match Qs with
+    | [::] => Some Q
+    | h :: t => if h == Q then merge_mq Q t
+                else None
+    end.
+
+  Definition merge_q (Q : seq MsgQ) :=
+    match Q with
+    | [::] => Some [::]
+    | h :: t => merge_mq h t
+    end.
+
+  Print project.
+
   Fixpoint q_proj G (p : role) : option (MsgQ * l_ty):=
     match G with
     | rg_end => Some ([::], l_end)
+    | rg_var v => Some ([::], l_var v)
+    | rg_rec G =>
+      match q_proj G p with
+      | Some (Q, P) =>
+        if P == l_var (Rvar.bv 0) then None else Some (Q, l_rec P)
+      | None => None
+      end
     | rg_msg m G =>
       match q_proj G p with
       | Some QP => if m.snd == m.rcv then None
@@ -54,41 +76,71 @@ Section TraceEquiv.
                              else Some QP
       | None => None
       end
-        (* )
     | rg_brn m K =>
-      let KL := map (fun X => (X.1, q_proj X.2 r)) K in
-    if m.snd == m.rcv
-    then None
-    else if m.snd == p
-         then ml_sel q K
-         else if q == r
-              then ml_brn p K
-              else merge_all K.
-
-      match q_proj G p with
-      | Some QP => if m.snd == m.rcv then None
-                   else if m.snd == p
-                        then Some (add_head (msg m) QP.1, QP.2)
-                        else if m.rcv == p
-                             then Some (QP.1, l_recv m.snd m.typ QP.2)
-                             else Some QP
+      match
+        (fix q_projK K : option (seq MsgQ * seq (lbl * l_ty)):=
+           match K with
+           | [::] => Some ([::], [::])
+           | lG :: K =>
+             match q_proj lG.2 p, q_projK K with
+             | Some QP, Some QK =>
+                 Some (QP.1 :: QK.1, (lG.1, QP.2) :: QK.2)
+             | _, _ => None
+             end
+           end
+        ) K
+      with
       | None => None
+      | Some (Q, K) =>
+        match merge_q Q with
+        | None => None
+        | Some Q =>
+          if m.snd == m.rcv then None
+          else if m.snd == p
+               then Some (Q, l_sel m.rcv K)
+               else if m.rcv == p
+                    then Some (Q, l_brn m.snd K)
+                    else match K with
+                         | [::] => None
+                         | h :: t => if all (fun X => h.2 == X.2) t
+                                     then Some (Q, h.2)
+                                     else None
+                         end
+        end
       end
-    | g_brn p K =>
-      let KL := map (fun X => (X.1, project X.2 r)) K in
-      project_brn p r KL *)
-    | _ => None
+    | rg_alt lb m K =>
+      match
+        (fix q_projK K : option (seq MsgQ * seq (lbl * l_ty)):=
+           match K with
+           | [::] => Some ([::], [::])
+           | lG :: K =>
+             match q_proj lG.2 p, q_projK K with
+             | Some QP, Some QK =>
+                 Some (QP.1 :: QK.1, (lG.1, QP.2) :: QK.2)
+             | _, _ => None
+             end
+           end
+        ) K
+      with
+      | None => None
+      | Some (Q, K) =>
+        match merge_q Q, lookup lb K with
+        | Some Q, Some G =>
+          if m.snd == m.rcv then None
+          else if m.snd == p
+               then Some (add_head (lab m lb) Q, G)
+               else if m.rcv == p
+                    then Some (Q, l_brn m.snd K)
+                    else match K with
+                         | [::] => None
+                         | h :: t => if all (fun X => h.2 == X.2) t
+                                     then Some (Q, h.2)
+                                     else None
+                         end
+        | _, _ => None
+        end
+      end
     end.
-
-  Definition project_brn (p : g_prefix) (r : role) (K : seq (lbl * option l_ty)) :=
-    let: ((p, q), t) := p in
-    if p == q
-    then None
-    else if p == r
-         then ml_sel q K
-         else if q == r
-              then ml_brn p K
-              else merge_all K.
 
   Definition q_union (Q1 Q2 : MsgQ) := Q1 ++ Q2.
 
@@ -105,15 +157,57 @@ Section TraceEquiv.
     q_project G (rg_parts G).
 
   Lemma g_trequiv G :
-    forall P,
+    forall (P : MsgQ * seq (role * l_ty)),
     q_projection G == Some P ->
     trace_equiv G P.
+  Proof.
+    rewrite /q_projection/trace_equiv.
   Admitted.
+
+  Lemma rgparts_init G :
+    rg_parts (init G) = participants G.
+  Proof.
+    elim/gty_ind2: G=>/=//.
+    + by move=> [[p q] ty] G/=->.
+    + move=> [[p q] ty] Gs /=/forall_member-Ih; do ! (congr cons).
+      congr seq.flatten; rewrite -map_comp/comp/=.
+      by apply/Fa_map_eq/forall_member => lG /(Ih lG).
+  Qed.
+
+
+  Lemma project_init G P :
+    projection G == Some P -> q_projection (init G) = Some ([::], P).
+  Proof.
+    rewrite /projection/q_projection rgparts_init; elim: (participants G) P.
+    - by move=>P /eqP-[<-].
+    - move=> a ps Ih/= P.
+      suff: forall L, project G a == Some L ->
+                      q_proj (init G) a == Some ([::], L).
+      {
+        case: (project G a)=>/=// L' /(_ L').
+        rewrite eq_refl=>/(_ is_true_true) =>/eqP->.
+        case: P=>//; first (by case: (project_all G ps)).
+        move=> lG P; move: (Ih P); case: (project_all G ps) =>// P' {Ih}H.
+        by move=>/eqP-[-> PP']; move: PP' H =>-> /(_ (eq_refl _))->/=.
+      }
+      move=> {Ih P ps}.
+      elim/gty_ind2: G=>//.
+      + move=> G Ih L/=; move: Ih.
+        case: (project G a)=>// L' /(_ L' (eq_refl _))/eqP->/=.
+        by rewrite -[Some _ == Some _]/(L' == _); case: ifP.
+      + move=> [[p q] ty] G/=; rewrite /ml_send/ml_recv.
+        case: (ifP (p == q))=>//.
+        case: (project G a) =>//;
+          last (by case: (ifP (p == a))=>//; case: (ifP (q == a))).
+        move=>L _ /(_ L (eq_refl _)) /eqP-> L'/=.
+        by (do ! case: ifP=>//).
+      + move=> [[p q] ty] K Ih/= L.
+  Admitted. (* TODO: Fix q_proj to simplify proof *)
 
   Theorem global_local_trequiv G :
     forall P,
     projection G == Some P ->
     trace_equiv (init G) ([::], P).
-  Admitted.
+  Proof. by move=>P /project_init/eqP; apply g_trequiv. Qed.
 
 End TraceEquiv.
